Trying to handle wait steps in pure WaitGroup protocol;
requires essentially having pure facts capture constraints imposed by
resources in the existing proof. E.g. after Wait2, need to have some
fact that survives across steps that implies that the counter is 0.

new/proof/sync2.v
@@ -119,7 +119,20 @@ Ltac word := first [
                | fail 1 "word could not solve goal"
                ].
 
+(* TODO: use for first abstraction. *)
+Local Definition enc (low high : w32) : w64 :=
+  word.add (word.slu (W64 (uint.Z high)) (W64 32)) (W64 (uint.Z low)).
 
+(* TODO: use for first abstraction. *)
+Local Ltac local_word :=
+  try apply word.unsigned_inj;
+  repeat try (
+      rewrite !word.unsigned_sru // in * ||
+      rewrite word.unsigned_add ||
+      rewrite word.unsigned_slu // ||
+      rewrite !Z.shiftr_div_pow2 // ||
+      rewrite Z.shiftl_mul_pow2 //
+    ); word.
 
 (* TODO: this is an abstraction of the physical state. *)
 Record Impl := mkImpl { v : w32; w : w32; sema : u32; }.
@@ -128,7 +141,9 @@ Global Instance settable : Settable _ :=
 Implicit Types s : Impl.
 
 Inductive ImplStep :=
-| Add1 (delta : w32) | Add2 | Add3.
+| Add1 (delta : w32) | Add2 | Add3
+| Wait1 (oldv oldw : w32) | Wait2.
+
 Implicit Type (l : ImplStep).
 
 Definition step_impl l s s' : Prop :=
@@ -136,6 +151,11 @@ Definition step_impl l s s' : Prop :=
   | Add1 delta => (s' = s <| v := word.add s.(v) delta |>)
   | Add2 => (s' = s <| v := W32 0 |> <| w := W32 0 |>)
   | Add3 => (s' = s <| sema := (word.add s.(sema) (W32 1)) |>)
+
+  | Wait1 oldv oldw => if decide (s.(v) = oldv ∧ s.(w) = oldw) then
+                        (s' = s <| w := (word.add oldw (W32 1)) |>)
+                      else s' = s
+  | Wait2 => (0 < uint.Z s.(sema)) ∧ (s' = s <| sema := word.sub s.(sema) (W32 1) |>)
   end.
 
 Record Spec := { counter : w32; }.
@@ -158,24 +178,8 @@ Definition next_add_aux l s s' a : AuxAdd :=
   | _ => AddNot
   end.
 
-(* TODO: use for first abstraction. *)
-Local Definition enc (low high : w32) : w64 :=
-  word.add (word.slu (W64 (uint.Z high)) (W64 32)) (W64 (uint.Z low)).
-
-(* TODO: use for first abstraction. *)
-Local Ltac local_word :=
-  try apply word.unsigned_inj;
-  repeat try (
-      rewrite !word.unsigned_sru // in * ||
-      rewrite word.unsigned_add ||
-      rewrite word.unsigned_slu // ||
-      rewrite !Z.shiftr_div_pow2 // ||
-      rewrite Z.shiftl_mul_pow2 //
-    ); word.
-
 Definition invariant s t a : Prop :=
   t.(counter) = s.(v) ∧ (* abstraction *)
-  0 ≤ sint.Z s.(v) ∧
   match a with
   | AddNeedToSignal => s.(v) = W32 0
   | _ => True
@@ -187,35 +191,61 @@ Lemma impl_invariant_Add1 delta s s' t a :
   invariant s t a →
   ∃ t', step_spec (Add delta) t t' ∧ invariant s' t' (next_add_aux (Add1 delta) s s' a).
 Proof.
-  intros Hpre Hstep Hinv. unfold invariant in *.
-  destruct s as [v w sema], s' as [v' w' sema'].
-  destruct t as [counter]. exists {|sync2.counter := v'|}. simpl in *.
+  intros Hpre Hstep Hinv. destruct s as [v w sema], s' as [v' w' sema'], t as [counter].
+  exists {|sync2.counter := v'|}. unfold invariant in *. simpl in *.
   unfold set in Hstep. simplify_eq. intuition; try word. by destruct decide.
 Qed.
 
 Lemma impl_invariant_Add2 s s' t a :
+  (* XXX: The precondition here is actually meant to denote ownership. *)
   a = AddNeedToSignal →
   step_impl Add2 s s' →
   invariant s t a →
   invariant s' t (next_add_aux (Add2) s s' a).
 Proof.
-  intros -> Hstep Hinv.
-  destruct s as [v w sema], s' as [v' w' sema'], t as [counter].
+  intros -> Hstep Hinv. destruct s as [v w sema], s' as [v' w' sema'], t as [counter].
   unfold invariant in *. simpl in *. unfold set in *. simpl in *. simplify_eq.
   intuition; subst; done.
 Qed.
 
 Lemma impl_invariant_Add3 s s' t a :
-  a = AddNeedToSignal →
-  step_impl Add2 s s' →
+  step_impl Add3 s s' →
   invariant s t a →
-  invariant s' t (next_add_aux (Add2) s s' a).
+  invariant s' t (next_add_aux (Add3) s s' a).
 Proof.
-  intros -> Hstep Hinv. unfold invariant in *.
-  destruct s as [v w sema], s' as [v' w' sema'].
-  destruct t as [counter]. simpl in Hstep. unfold set in *. simpl in *. simplify_eq.
+  intros Hstep Hinv. destruct s as [v w sema], s' as [v' w' sema'], t as [counter].
+  unfold invariant in *. simpl in *. unfold set in *. simpl in *. simplify_eq.
   intuition; subst; done.
 Qed.
+
+Lemma impl_invariant_Wait1 oldv oldw s s' t a :
+  sint.Z oldv ≠ 0 →
+  step_impl (Wait1 oldv oldw) s s' →
+  invariant s t a →
+  invariant s' t (next_add_aux (Wait1 oldv oldw) s s' a).
+Proof.
+  intros Hstep Hinv. destruct s as [v w sema], s' as [v' w' sema'], t as [counter].
+  unfold invariant in *. simpl in *.
+  unfold set in *. simpl in *. destruct decide; simplify_eq.
+  all: intuition; subst; done.
+Qed.
+
+Lemma impl_invariant_Wait2 s s' t a :
+  step_impl Wait2 s s' →
+  invariant s t a →
+  ∃ t', step_spec Wait t t' ∧
+        invariant s' t' (next_add_aux Wait2 s s' a).
+Proof.
+  intros Hstep Hinv. exists t. destruct s as [v w sema], s' as [v' w' sema'], t as [counter].
+  unfold invariant in *. simpl in *.
+  unfold set in *. simpl in *. destruct Hstep as [? Hstep].
+  simplify_eq. split_and!; try done.
+  {
+Abort.
+(* Need invariant to imply that counter = 0 in this case. But, that's not enough:
+   need to walk away with a fact that says the counter will remain zero until
+   the Wait() call returns.
+   I.e. want some sort of ownership. *)
 
 
 (* Q: steps are constrained by preconditions on API functions. How does that show up here? *)
